Merge operatorTheory into combinTheory
This was far too small a theory to live an independent existence.  It
was included by listTheory so the constant name-space contamination
isn't any different for eventual clients.

src/combin/combinScript.sml
@@ -289,6 +289,71 @@ val literal_case_FORALL_ELIM = store_thm(
     FIRST_X_ASSUM MATCH_MP_TAC THEN REFL_TAC
   ]);
 
+(* ----------------------------------------------------------------------
+    Predicates on functions
+   ---------------------------------------------------------------------- *)
+
+val ASSOC_DEF = new_definition("ASSOC_DEF",
+  ``
+    ASSOC (f:'a->'a->'a) <=> (!x y z. f x (f y z) = f (f x y) z)
+  ``);
+
+val COMM_DEF = new_definition("COMM_DEF",
+  ``
+     COMM (f:'a->'a->'b) <=> (!x y. f x y = f y x)
+  ``);
+
+val FCOMM_DEF = new_definition("FCOMM_DEF",
+  ``
+    FCOMM (f:'a->'b->'a) (g:'c->'a->'a) <=> (!x y z.  g x (f y z) = f (g x y) z)
+  ``);
+
+val RIGHT_ID_DEF = new_definition("RIGHT_ID_DEF",
+  ``
+    RIGHT_ID (f:'a->'b->'a) e <=> (!x. f x e = x)
+  ``);
+
+val LEFT_ID_DEF = new_definition("LEFT_ID_DEF",
+  ``
+    LEFT_ID (f:'a->'b->'b) e <=> (!x. f e x = x)
+  ``);
+
+val MONOID_DEF = new_definition("MONOID_DEF",
+  ``
+    MONOID (f:'a->'a->'a) e <=>
+             ASSOC f /\ RIGHT_ID f e /\ LEFT_ID f e
+  ``);
+
+(* ======================================================================== *)
+(*  Theorems about operators                                                *)
+(* ======================================================================== *)
+
+val ASSOC_CONJ = store_thm ("ASSOC_CONJ", ``ASSOC $/\``,
+  REWRITE_TAC[ASSOC_DEF,CONJ_ASSOC]);
+
+val ASSOC_SYM = save_thm ("ASSOC_SYM",
+  CONV_RULE
+    (STRIP_QUANT_CONV (RHS_CONV (STRIP_QUANT_CONV SYM_CONV)))
+    ASSOC_DEF);
+
+
+val ASSOC_DISJ = store_thm ("ASSOC_DISJ",
+  ``ASSOC $\/``,
+  REWRITE_TAC[ASSOC_DEF,DISJ_ASSOC]);
+
+val FCOMM_ASSOC = store_thm ("FCOMM_ASSOC",
+  ``!f: 'a->'a->'a. FCOMM f f = ASSOC f``,
+  REWRITE_TAC[ASSOC_DEF,FCOMM_DEF]);
+
+val MONOID_CONJ_T = store_thm ("MONOID_CONJ_T",
+  ``MONOID $/\ T``,
+  REWRITE_TAC[MONOID_DEF,CONJ_ASSOC, LEFT_ID_DEF,ASSOC_DEF,RIGHT_ID_DEF]);
+
+val MONOID_DISJ_F = store_thm ("MONOID_DISJ_F",
+  ``MONOID $\/ F``,
+  REWRITE_TAC[MONOID_DEF,DISJ_ASSOC,
+              LEFT_ID_DEF,ASSOC_DEF,RIGHT_ID_DEF]);
+
 (*---------------------------------------------------------------------------*)
 (*  Tag combinator equal to K. Used in generating ML from HOL                *)
 (*---------------------------------------------------------------------------*)
